cleanup libheap

pretty/LibHeap.v
@@ -10,7 +10,7 @@
 
 Set Implicit Arguments.
 From TLC Require Import LibTactics LibReflect LibList LibListAssoc
-  LibSet LibListExec.
+  LibSet LibListExec LibVar.
 Generalizable Variable K V.
 
 
@@ -26,183 +26,20 @@ Class Decidable (P:Prop) := decidable_make {
   decide : bool;
   decide_spec : decide = isTrue P }.
 
-Hint Rewrite @decide_spec : rew_refl.
 Arguments decide P {Decidable}.
 
-(** Notation [ifb P then x else y] can be used for
+(** The tactic [rew_bool_eq], used by [case_if], is extended
+    with support for [decide] *)
+
+Hint Rewrite (@decide_spec) : rew_bool_eq.
+
+(** The notation [ifb P then x else y] can be used for
     testing a proposition [P] for which there exists an
     instance of [Decidable P]. *)
 
 Notation "'ifb' P 'then' v1 'else' v2" :=
   (if decide P then v1 else v2)
   (at level 200, right associativity) : type_scope.
-
-(** In classical logic, any proposition is decidable; of course,
-    we do not want to use this lemma as an instance because
-    it cannot be extracted to executable code. *)
-
-Lemma prop_decidable : forall (P:Prop), Decidable P.
-Proof using. intros. applys~ decidable_make (isTrue P). Qed.
-
-(** In constructive logic, any proposition with a proof of
-    that is constructively true or false is decidable. *)
-
-Definition sumbool_decidable : forall (P:Prop),
-  {P}+{~P} -> Decidable P.
-Proof using.
-  introv H. applys decidable_make
-    (match H with left _ => true | right _ => false end).
-  destruct H; rew_bool_eq~.
-Defined.
-
-(*
-
-Definition decidable_sumbool : forall P : Prop,
-    Decidable P -> {P}+{~P}.
-Proof using.
-  introv D. destruct (decide P) eqn: H. rew_bool_eq in H; [left*|right*].
-
-Defined.
-
-(** [sumbool_decidable] and [decidable_sumbool] just wrap their
-    property as expected. *)
-
-Lemma sumbool_decidable_decidable_sumbool : forall P (d : {P}+{~P}),
-  decidable_sumbool (sumbool_decidable d) = d.
-Proof using.
-  introv. unfolds.
-  asserts R1: (forall (d : bool) B C C1 C2,
-    d ->
-    (if d as b return (d = b -> B) then
-      fun H => C1 H
-    else fun H => C2 H) eq_refl = C ->
-    exists E, C1 E = C).
-   clear. introv D Eq. destruct d; tryfalse. eexists. apply Eq.
-  lets R1': (rm R1) (@decide P (sumbool_decidable d)).
-  asserts R2: (forall (d : bool) B C C1 C2,
-    !d ->
-    (if d as b return (d = b -> B) then
-      fun H => C1 H
-    else fun H => C2 H) eq_refl = C ->
-    exists E, C2 E = C).
-   clear. introv D Eq. destruct d; tryfalse. eexists. apply Eq.
-  lets R2': (rm R2) (@decide P (sumbool_decidable d)).
-  unfold sumbool_decidable. case_if as I.
-   forwards (E&Eq): R1'.
-     rewrite decide_spec. rew_refl*.
-     reflexivity.
-    rewrite <- Eq. fequals.
-   forwards (E&Eq): R2'.
-     rewrite decide_spec. rew_refl*.
-     reflexivity.
-    rewrite <- Eq. fequals.
-Qed.
-
-
-Global Instance Decidable_impl : forall A B : Prop,
-    Decidable A -> Decidable B -> Decidable (A -> B).
-  introv (da&Ha) (db&Hb).
-  destruct da; destruct db; fold_bool; rew_refl in *;
-    ((apply decidable_make with true; solve [ fold_bool; rew_refl* ]) ||
-     (apply decidable_make with false; solve [ fold_bool; rew_refl* ])).
-Defined.
-
-Global Instance Decidable_equiv : forall A B : Prop,
-    (A <-> B) -> Decidable A -> Decidable B.
-  introv E. apply prop_ext in E. substs~.
-Defined.
-
-(** Extending the [case_if] tactic to support [if decide] *)
-
-Lemma Decidable_dec : forall (P:Prop) {H: Decidable P} (A:Type) (x y:A),
-  exists (Q : {P}+{~P}),
-  (if decide P then x else y) = (if Q then x else y).
-Proof using.
-  intros. exists (classicT P).
-  rewrite decide_spec.
-  tautotest P; case_if as C; case_if as C';
-  first [ rewrite isTrue_True in C
-        | rewrite isTrue_False in C
-        | idtac ]; autos*; false*.
-Qed.
-
-Ltac case_if_on_tactic_core E Eq ::=
-  match E with
-  | @decide ?P ?M =>
-      let Q := fresh in let Eq := fresh in
-      forwards (Q&Eq): (@Decidable_dec P M);
-      rewrite Eq in *; clear Eq; destruct Q
-  | _ =>
-    match type of E with
-    | {_}+{_} => destruct E as [Eq|Eq]; try subst_hyp Eq
-    | _ => let X := fresh in
-           sets_eq <- X Eq: E;
-           destruct X
-    end
-  end.
-
-(** Rewriting lemma *)
-
-Lemma istrue_decide : forall `{Decidable P},
-  istrue (decide P) = P.
-Proof using. intros. rew_refl~. Qed.
-
-Lemma decide_prove : forall `{Decidable P},
-  P -> istrue (decide P).
-Proof using. intros. rewrite~ istrue_decide. Qed.
-
-Lemma decide_def : forall `{Decidable P},
-  (decide P) = (If P then true else false).
-Proof using. intros. rewrite decide_spec. rewrite isTrue_to_if. case_if*. Qed.
-
-Lemma decide_cases : forall `{Decidable P},
-  (P /\ decide P = true) \/ (~ P /\ decide P = false).
-Proof using. intros. rewrite decide_spec. rewrite isTrue_to_if. case_if*. Qed.
-
-(** Dedicability instances *)
-
-Global Instance true_decidable : Decidable True.
-Proof using. applys decidable_make true. rew_refl~. Qed.
-
-Global Instance false_decidable : Decidable False.
-Proof using. applys decidable_make false. rew_refl~. Qed.
-
-Global Instance bool_decidable : forall (b : bool), Decidable (b).
-Proof using. introv. applys (@decidable_make (istrue b) b). rew_refl~. Qed.
-
-Global Instance not_decidable : forall (P : Prop),
-  Decidable P -> Decidable (~ P).
-Proof using.
-  (* --TODO: cleanup proof *)
-  introv [dec spec]. applys decidable_make (neg dec).
-  rew_refl. rewrite~ spec.
-Qed.
-
-Global Instance or_decidable : forall (P Q : Prop),
-  Decidable P -> Decidable Q ->
-  Decidable (P \/ Q).
-Proof using.
-  intros. applys decidable_make (decide P || decide Q).
-  rew_refl. subst~.
-Qed.
-
-Global Instance and_decidable : forall P Q,
-  Decidable P -> Decidable Q ->
-  Decidable (P /\ Q).
-Proof using.
-  intros. applys decidable_make (decide P && decide Q).
-  rew_refl. subst~.
-Qed.
-
-Global Instance If_dec : forall P Q R,
-  Decidable P -> Decidable Q -> Decidable R ->
-  Decidable (If P then Q else R).
-Proof using.
-  intros. applys decidable_make (if decide P then decide Q else decide R).
-  rew_refl. subst~.
-Qed.
-
-*)
 
 
 (* ********************************************************************** *)
@@ -215,13 +52,6 @@ Class Comparable (A:Type) := make_comparable {
   comparable : forall (x y:A), Decidable (x = y) }.
 
 Hint Resolve comparable : typeclass_instances.
-
-(** In classical logic, any type is comparable; of course,
-    we do not want to use this lemma as an instance because
-    it cannot be extracted to executable code. *)
-
-Lemma type_comparable : forall (A:Type), Comparable A.
-Proof using. constructor. intros. applys~ prop_decidable. Qed.
 
 (** [Comparable] can be proved by exhibiting a boolean
     comparison function *)
@@ -247,28 +77,30 @@ Proof using.
   case_if; rew_bool_eq*.
 Qed.
 
-(** Comparison for booleans *)
+(** Comparison for bool *)
 
-Instance bool_comparable : Comparable bool.
+Global Instance comparable_bool : Comparable bool.
 Proof using.
   applys (comparable_beq Bool.eqb).
   destruct x; destruct y; simpl; rew_bool_eq; auto_false*.
 Qed.
 
-(*
-Global Instance prop_eq_decidable : forall P Q,
-  Decidable P -> Decidable Q ->
-  Decidable (P = Q).
-Proof using.
-  intros. applys decidable_make (decide (decide P = decide Q)).
-  extens. rew_bool_eq in *.
-  iff E.
-    do 2 rewrite isTrue_to_if in E.
-     extens. case_if; case_if; auto_false*.
-    subst*.
-Qed.
-*)
+(** Comparison for nat *)
 
+Global Instance comparable_nat : Comparable nat.
+Proof using.
+  applys (comparable_beq Nat.eqb).
+  intros x. induction x; intros y; destruct y; simpl; rew_bool_eq; auto_false*.
+  rewrite IHx. iff M. { auto. } { inverts* M. }
+Qed.
+
+(** Comparison for var *)
+
+Global Instance comparable_var : Comparable var.
+Proof using.
+  applys (comparable_beq var_compare). intros.
+  rewrite var_compare_eq. rew_bool_eq*.
+Qed.
 
 
 (***********************************************************)
@@ -285,11 +117,10 @@ Parameter heap : Type -> Type -> Type.
 (** Required operations *)
 
 Section HeapDef.
-Variables K V : Type.
-Parameter empty : heap K V.
-Parameter write : heap K V -> K -> V -> heap K V.
-Parameter rem : forall `{Comparable K} V, heap K V -> K -> heap K V.
-Parameter read_opt : forall `{Comparable K} V, heap K V -> K -> option V.
+Parameter empty : forall K V, heap K V.
+Parameter write : forall K V, heap K V -> K -> V -> heap K V.
+Parameter rem : forall K `{Comparable K} V, heap K V -> K -> heap K V.
+Parameter read_opt : forall K `{Comparable K} V, heap K V -> K -> option V.
 End HeapDef.
 
 (** Required properties *)
@@ -306,7 +137,7 @@ Parameter read_opt_empty : forall k,
 Parameter read_opt_write : forall k k' v h,
   read_opt (write h k' v) k = ifb k = k' then Some v else read_opt h k.
 
-Parameter read_opt_rem : forall k k' v h,
+Parameter read_opt_rem : forall k k' h,
   read_opt (rem h k') k = ifb k = k' then None else read_opt h k.
 
 End HeapProp.
@@ -324,7 +155,7 @@ Lemma filter_eq' : forall A (P:A->Prop) (p:A->bool) l,
   filter p l = LibList.filter P l.
 Proof using. intros. applys* filter_eq. Qed.
 
-Module HeapList : HeapSpec.
+Module Export HeapImpl : HeapSpec.
 
 (** Realize Type *)
 
@@ -333,7 +164,7 @@ Definition heap K V := list (K*V).
 (** Realize operations *)
 
 Section HeapDef.
-Variables K V : Type.
+Context `{Comparable K} (V : Type).
 Implicit Types k : K.
 Implicit Types v : V.
 Implicit Types h : heap K V.
@@ -344,10 +175,10 @@ Definition empty : heap K V :=
 Definition write h k v :=
   (k, v) :: h.
 
-Definition rem `{Comparable K} h k :=
+Definition rem h k :=
   LibListExec.filter (fun '(k',v) => ! (decide (k' = k))) h.
 
-Fixpoint read_opt `{Comparable K} h k :=
+Fixpoint read_opt h k :=
   match h with
   | nil => None
   | (k', v) :: h' => ifb k = k' then Some v else read_opt h' k
@@ -379,9 +210,7 @@ Proof using.
   { intros (ki,vi). simpl. rewrite decide_spec. rewrite* isTrue_not. }
 Qed.
 
-Hint Rewrite (@decide_spec) : rew_bool_eq.
-
-Lemma read_opt_rem : forall k k' v h,
+Lemma read_opt_rem : forall k k' h,
   read_opt (rem h k') k = ifb k = k' then None else read_opt h k.
 Proof using HK.
   intros. rewrite rem_eq_filter. case_if.
@@ -395,499 +224,288 @@ Qed.
 
 End HeapProp.
 
-End HeapList.
-
-
-
-
+End HeapImpl.
 
 
 (***********************************************************)
 (***********************************************************)
 (***********************************************************)
-(* Note: move to LibListAssocExec *)
+(** Derived properties of any heap implementation *)
 
-Generalizable Variable A B.
+Module Heap.
+Include HeapImpl.
 
-Fixpoint assoc `{Comparable A} `{Inhab B} k (l:list (A*B)) : B :=
-  match l with
-  | nil => arbitrary
-  | (x, v) :: l' => ifb x = k then v else assoc k l'
-  end.
+(** Additional operators *)
 
-
-Module HeapList : HeapSpec.
-
-Definition heap K V := list (K*V).
-
-Section HeapDefs.
-Context `{Comparable K} `{Inhab V}.
+Section HeapMoreDef.
+Context `{Comparable K} (V : Type).
+Implicit Types k : K.
+Implicit Types v : V.
 Implicit Types h : heap K V.
 
-Definition empty : heap K V := nil.
+Definition indom_dec h k :=
+  match read_opt h k with
+  | None => false
+  | Some v => true
+  end.
 
-Definition dom h : set K :=
-  fold_right (fun p acc => acc \u \{fst p}) \{} h.
+Definition indom h k :=
+  match read_opt h k with
+  | None => False
+  | Some v => True
+  end.
+
+Definition read `{Inhab V} h k :=
+  match read_opt h k with
+  | None => arbitrary
+  | Some v => v
+  end.
 
 Definition binds h k v :=
-  Assoc k v h.
-
-Definition to_list h :=
-  h.
-
-Definition read h k :=
-  assoc k h.
-
-Definition write h k v :=
-  (k, v) :: h.
-
-Definition rem K `{Comparable K} V (h : heap K V) k :=
-  LibList.filter (fun p => ifb (fst p) = k then false else true) h.
-
-Definition indom h r :=
-  List.Exists (fun '(k,v) => k = r) h.
-  (*(r \in dom h).*)
-
-Fixpoint read_opt (h : heap K V) k :=
-  match l with
-  | nil => None
-  | (x, v) :: h' => ifb x = k then Some v else read_opt h' k
+  match read_opt h k with
+  | None => False
+  | Some v' => (v = v')
   end.
 
-End HeapDefs.
+End HeapMoreDef.
 
-Arguments empty {K} {V}.
+(** Properties of additional operators *)
 
-Generalizable Variable A.
-
-Fixpoint mem_assoc B `{Comparable A} k (l : list (A * B)) : bool :=
-  match l with
-  | nil => false
-  | (x, _) :: l' => decide (x = k) || mem_assoc k l'
-  end.
-
-Definition indom_dec `{Comparable K} V (h:heap K V) (k:K) : bool :=
-  mem_assoc k h.
-
-(** Properties *)
-
-Section HeapParameters.
-Context (K:Type) (HK: Comparable K) (V:Type) (IV: Inhab V).
+Section HeapMoreProp.
+Context (K:Type) (HK:Comparable K) (V:Type) (IV:Inhab V).
+Implicit Types k : K.
+Implicit Types v : V.
 Implicit Types h : heap K V.
 
-Lemma dom_empty :
-  dom (@empty K V) = \{}.
-Proof using. auto. Qed.
-
-Lemma dom_write : forall h r v,
-  dom (write h r v) = dom h \u \{r}.
-Proof. intros. unfold dom, write. rew_list. auto. Qed.
-
-Lemma indom_equiv_binds : forall h k,
-  indom h k = (exists v, binds h k v).
-Proof using.
-  intros. unfold indom, binds, dom.
-Admitted.
-
-(r \in dom h)
-
-Lemma binds_equiv_read : forall h k,
-  indom h k -> (forall v, (binds h k v) = (read h k = v)).
-Proof using HK IV.
-Admitted. (* File will be soon deprecated *)
-
-Arguments binds_equiv_read : clear implicits.
-
-
-Lemma binds_write_eq : forall h k v,
-  binds (write h k v) k v.
-Proof. unfolds @binds, @write. intros. constructors. Qed.
-
-Lemma binds_write_neq : forall h k v k' v',
-  binds h k v -> k <> k' ->
-  binds (write h k' v') k v.
-Proof. unfolds @binds, @write. intros. constructors~. Qed.
-
-Lemma binds_write_inv : forall h k v k' v',
-  binds (write h k' v') k v ->
-  (k = k' /\ v = v') \/ (k <> k' /\ binds h k v).
-Proof. unfolds @binds, @write. introv M. inverts* M. Qed.
-
-Lemma binds_rem : forall h k k' v,
-  binds h k v -> k <> k' -> binds (rem h k') k v.
-Proof using HK.
-Admitted. (* File will be soon deprecated *)
-
-Lemma binds_rem_inv : forall h k v k',
-  binds (rem h k') k v -> k <> k' /\ binds h k v.
-Proof using HK.
-Admitted. (* File will be soon deprecated *)
-
-
-Lemma not_indom_rem : forall h k,
-  ~ indom (rem h k) k.
-Proof using HK.
-Admitted. (* File will be soon deprecated *)
-
-
-Lemma binds_equiv_read_opt : forall h k v,
-  (binds h k v) = (read_opt h k = Some v).
-Admitted. (* File will be soon deprecated *)
-
-(*
-Proof using. clear IV.
-  unfolds @binds. introv. extens.
-  induction h as [|(x&v0)].
-   splits ; intro N ; invert* N.
-   simpl. case_if.
-     subst. splits ; intro N ; inverts* N. constructors.
-     splits ; intro N.
-      inverts* N.
-      constructors*.
-Qed.
-*)
-
-Lemma not_indom_equiv_read_opt : forall h k,
-  (~ indom h k) = (read_opt h k = None).
-Proof using IV.
-Admitted. (* File will be soon deprecated *)
-(*
-  introv. apply* injective_not. rew_logic. rewrite indom_equiv_binds.
-  splits ; intro N.
-   lets (v & B): rm N.
-    rewrite binds_equiv_read_opt in B. rewrite* B. discriminate.
-   asserts (v & E): (exists v, read_opt h k = Some v).
-     destruct* @read_opt.
-    rewrite* <- binds_equiv_read_opt in E.
-Qed.
-*)
-
-Lemma read_opt_def : forall h k,
-  read_opt h k = (If indom h k then Some (read h k) else None).
-Proof using.
-(* --TODO
-  introv. cases_if.
-   rewrite* <- binds_equiv_read_opt.
-    rewrites* binds_equiv_read.
-   rewrite* <- @not_indom_equiv_read_opt.
-*)
-Admitted. (* File will be soon deprecated *)
-
-(* --TODO: move *)
-
-
-
-Lemma indom_dec_spec : forall (CK:Comparable K) V (h:heap K V) k,
-  indom_dec h k = isTrue (indom h k).
-Proof.
-  intros. unfold indom, dom, indom_dec.
-  induction h as [|[k' v'] h]; simpl; rew_listx.
-  rewrite in_empty_eq. rew_bool_eq~.
-  rewrite in_union_eq. rewrite in_single_eq. rewrite IHh.
-   extens. rew_bool_eq*.
-Admitted. (* File will be soon deprecated *)
-
-End HeapParameters.
-
-Lemma indom_decidable : forall K (CK:Comparable K) V (h:heap K V) k,
-  Decidable (indom h k).
-Proof.
-  intros. applys decidable_make (indom_dec h k).
-  applys indom_dec_spec.
-Admitted. (* File will be soon deprecated *)
-
-End HeapList.
-
-Export HeapList.
-
-
-(***********************************************************)
-(** Derived facts true for all heap implementations *)
-
-Global Instance Inhab_heap : forall (K V : Type), Inhab (heap K V).
-Proof using. introv. apply (Inhab_of_val empty). Qed.
-
-Section HeapFacts.
-Context `{HK:Comparable K} `{HV:Inhab V}.
-Implicit Types h : heap K V.
-
-(** indom *)
-
-Lemma indom_binds : forall h k,
-  indom h k -> exists v, binds h k v.
-Proof using. introv H. rewrite~ @indom_equiv_binds in H. Qed.
-
-Lemma binds_indom : forall h k v,
-  binds h k v -> indom h k.
-Proof using. introv H. rewrite* @indom_equiv_binds. Qed.
-
-(** binds-func *)
-
-Lemma binds_functional : forall h k v v',
-  binds h k v -> binds h k v' -> v = v'.
-Proof using HK HV.
-  introv B1 B2. forwards: binds_indom B1. forwards: binds_indom B2.
-  rewrite (@binds_equiv_read K HK V HV) in B1, B2; auto. congruence.
-Qed.
-
-(** read--binds *)
-
-Lemma binds_read : forall h k v,
-  binds h k v -> read h k = v.
-Proof using. introv H. rewrite~ <- binds_equiv_read. apply* binds_indom. Qed.
-
-Lemma read_binds : forall h k v,
-  read h k = v -> indom h k -> binds h k v.
-Proof using. introv H D. erewrite binds_equiv_read; auto. Qed.
-
-(** read-write *)
-
-Lemma read_write_eq : forall h k v,
-  read (write h k v) k = v.
-Proof using. introv. apply binds_read. apply binds_write_eq. Qed.
-
-Lemma read_write_neq : forall h k k' v',
-  indom h k -> k <> k' -> read (write h k' v') k = read h k.
-Proof using.
-  introv. rewrite indom_equiv_binds. introv [v B] N.
-  rewrite (binds_read B).
-  forwards B': @binds_write_neq B N. rewrite~ (binds_read B').
-Qed.
-
-(** indom-write *)
-
-Lemma indom_write_eq : forall h k v,
-  indom (write h k v) k.
-Proof using.
-  intros. rewrite indom_equiv_binds. exists v.
-  apply* @binds_write_eq.
-Qed.
-
-Lemma indom_write : forall h k k' v',
-  indom h k -> indom (write h k' v') k.
-Proof using.
-  introv. do 2 rewrite indom_equiv_binds.
-  introv [v B]. tests: (k = k').
-    subst. exists v'. apply* @binds_write_eq.
-    exists v. apply* @binds_write_neq.
-Qed.
-
-Lemma indom_write_inv : forall h k k' v',
-  indom (write h k' v') k -> k <> k' -> indom h k.
-Proof using.
-  introv. do 2 rewrite indom_equiv_binds.
-  introv [v B] N. lets [[? ?]|[? ?]]: @binds_write_inv B.
-  false. eauto.
-Qed.
-
-(** binds-write *)
-
-Lemma binds_write_eq_inv : forall h k v v',
-  binds (write h k v') k v -> v = v'.
-Proof using.
-  introv B. lets [[? ?]|[? ?]]: @binds_write_inv B; auto_false.
-Qed.
-
-Lemma binds_write_neq_inv : forall h k v k' v',
-  binds (write h k' v') k v -> k <> k' -> binds h k v.
-Proof using.
-  introv B. lets [[? ?]|[? ?]]: @binds_write_inv B; auto_false.
-Qed.
-
-(** indom-rem *)
-
-Lemma indom_rem : forall h k k',
-  indom h k -> k <> k' -> indom (rem h k') k.
-Proof using.
-  introv. do 2 rewrite indom_equiv_binds.
-  introv [v B] N. exists v. apply* @binds_rem.
-Qed.
-
-Lemma indom_rem_inv : forall h k k',
-  indom (rem h k) k' -> k <> k' /\ indom h k'.
-Proof using.
-  introv. do 2 rewrite indom_equiv_binds.
-  introv [v B]. lets [? ?]: @binds_rem_inv B. eauto.
-Qed.
-
-(** read-rem *)
-
-Lemma read_rem_neq : forall h k k',
-  indom h k -> k <> k' -> read (rem h k') k = read h k.
-Proof using HK HV.
-  introv. rewrite indom_equiv_binds. introv [v B] N.
-  rewrite (binds_read B).
-  forwards B': @binds_rem B N. rewrite~ (binds_read B').
-Qed.
-
-(** indom-empty, binds-empty *)
+(** Properties of [indom] on [empty] *)
 
 Lemma not_indom_empty : forall k,
   ~ indom (@empty K V) k.
-Proof using HV.
-  introv H. unfold indom in H. rewrite dom_empty in H.
-  rew_set in H. eauto.
+Proof using. intros. unfold indom. rewrite* read_opt_empty. Qed.
+
+(** Properties of [indom] on [write] *)
+
+Lemma indom_write_eq : forall k k' v h,
+  indom (write h k' v) k = ((k = k') \/ indom h k).
+Proof using HK IV. (*  why using IV? *)
+  intros. extens. unfold indom. rewrite read_opt_write.
+  destruct (read_opt h k); case_if; case_if; rew_bool_eq in *; subst*.
 Qed.
+
+Lemma indom_write_same : forall h k v,
+  indom (write h k v) k.
+Proof using HK IV. intros. rewrite* indom_write_eq. Qed.
+
+Lemma indom_write : forall h k k' v',
+  indom h k ->
+  indom (write h k' v') k.
+Proof using HK IV. intros. rewrite* indom_write_eq. Qed.
+
+Lemma indom_write_inv_neq : forall h k k' v',
+  indom (write h k' v') k ->
+  k <> k' ->
+  indom h k.
+Proof using HK IV. introv M N. rewrite* indom_write_eq in M. Qed.
+
+(** Properties of [indom] on [rem] *)
+
+Lemma indom_rem_eq : forall k k' h,
+  indom (rem h k') k = ((k <> k') /\ indom h k).
+Proof using HK IV.
+  intros. extens. unfold indom. rewrite read_opt_rem.
+  destruct (read_opt h k); case_if; case_if; rew_bool_eq in *; subst*.
+Qed.
+
+Lemma indom_rem : forall h k k',
+  indom h k ->
+  k <> k' ->
+  indom (rem h k') k.
+Proof using HK IV. intros. rewrite* indom_rem_eq. Qed.
+
+Lemma indom_rem_inv : forall h k k',
+  indom (rem h k) k' ->
+  k <> k' /\ indom h k'.
+Proof using HK IV. introv M. rewrite* indom_rem_eq in M. Qed.
+
+Lemma not_indom_rem : forall h k,
+  ~ indom (rem h k) k.
+Proof using HK IV. intros. rewrite* indom_rem_eq. Qed.
+
+
+(** Properties of [indom] on [decide] *)
+
+Global Instance indom_decidable : forall `{Comparable K} V (h:heap K V) k,
+  Decidable (indom h k).
+Proof using HK.
+  intros. applys decidable_make (indom_dec h k). unfold indom_dec, indom.
+  destruct (read_opt h k); rew_bool_eq*.
+Qed.
+
+(** Properties of [read] on [write] *)
+
+Lemma read_write : forall k k' v h,
+  indom h k ->
+  read (write h k' v) k = If (k = k') then v else read h k.
+Proof using HK IV.
+  introv _. unfold read. rewrite read_opt_write. repeat case_if*.
+Qed.
+
+Lemma read_write_same : forall h k v,
+  indom h k ->
+  read (write h k v) k = v.
+Proof using HK IV. intros. rewrite* read_write. case_if*. Qed.
+
+Lemma read_write_neq : forall h k k' v,
+  indom h k ->
+  k <> k' ->
+  read (write h k' v) k = read h k.
+Proof using HK IV. intros. rewrite* read_write. case_if*. Qed.
+
+(** Properties of [read] on [rem] *)
+
+Lemma read_rem : forall k k' h,
+  indom h k ->
+  k <> k' ->
+  read (rem h k') k = read h k.
+Proof using HK.
+  intros. unfold read. rewrite read_opt_rem. case_if*.
+Qed.
+
+(** Properties of [binds]: functional *)
+
+Lemma binds_functional : forall h k v v',
+  binds h k v ->
+  binds h k v' ->
+  v = v'.
+Proof using.
+  introv M1 M2. unfold binds in *. destruct (read_opt h k); subst*.
+Qed.
+
+(** Properties of [binds] on [indom] *)
+
+Lemma indom_eq_exists_binds : forall h k,
+  indom h k = (exists v, binds h k v).
+Proof using.
+  intros. extens. unfold indom, binds. destruct (read_opt h k).
+  { autos*. } { iff ? (?&?); false. }
+Qed.
+
+Lemma indom_inv_binds : forall h k,
+  indom h k ->
+  exists v, binds h k v.
+Proof using. introv M. rewrite* indom_eq_exists_binds in M. Qed.
+
+Lemma binds_indom : forall h k v,
+  binds h k v ->
+  indom h k.
+Proof using. introv H. rewrite* indom_eq_exists_binds. Qed.
+
+(** Properties of [binds] on [read_opt] *)
+
+Lemma binds_eq_read_opt : forall h k v,
+  binds h k v = (read_opt h k = Some v).
+Proof using.
+  intros. extens. unfold binds, read. destruct (read_opt h k).
+  { iff M. { subst*. } { inverts* M. } }
+  { iff; false. }
+Qed.
+
+Lemma binds_inv_read_opt : forall h k v,
+  binds h k v ->
+  read_opt h k = Some v.
+Proof using. introv M. rewrite* binds_eq_read_opt in M. Qed.
+
+Lemma binds_of_read_opt : forall h k v,
+  read_opt h k = Some v ->
+  binds h k v.
+Proof using. intros. rewrite* binds_eq_read_opt. Qed.
+
+Lemma not_binds_of_read_opt : forall h k,
+  read_opt h k = None ->
+  forall v, ~ binds h k v.
+Proof using. introv E. intros. rewrite* binds_eq_read_opt. rewrite E; auto_false. Qed.
+
+(** Properties of [binds] on [read] *)
+
+Lemma binds_eq_indom_read : forall h k v,
+  binds h k v = (indom h k /\ read h k = v).
+Proof using. intros. extens. unfold binds, read, indom. destruct* (read_opt h k). Qed.
+
+Lemma binds_eq_read_of_indom : forall h k,
+  indom h k ->
+  (forall v, (binds h k v) = (read h k = v)).
+Proof using. introv M. extens. rewrite* binds_eq_indom_read. Qed.
+
+Lemma binds_inv_read : forall h k v,
+  binds h k v ->
+  read h k = v.
+Proof using. introv M. rewrite* binds_eq_indom_read in M. Qed.
+
+Lemma binds_of_read_indom : forall h k v,
+  read h k = v ->
+  indom h k ->
+  binds h k v.
+Proof using. intros. rewrite* binds_eq_indom_read. Qed.
+
+(** Properties of [binds] on [empty] *)
 
 Lemma not_binds_empty : forall k v,
   ~ binds (@empty K V) k v.
-Proof using HV. introv H. eapply not_indom_empty. apply* binds_indom. Qed.
+Proof using. intros. unfold binds. rewrite* read_opt_empty. Qed.
 
-(** binds--read_opt **)
+(** Properties of [binds] on [write] *)
 
-Lemma binds_read_opt : forall h k v,
-  binds h k v -> read_opt h k = Some v.
-Proof using HV. introv. rewrite* <- @binds_equiv_read_opt. Qed.
+Lemma binds_write_eq : forall h k v k' v',
+    binds (write h k' v') k v
+  = If k = k' then v = v' else binds h k v.
+Proof using. intros. unfold binds. rewrite* read_opt_write. repeat case_if*. Qed.
 
-Lemma read_opt_binds : forall h k v,
-  read_opt h k = Some v -> binds h k v.
-Proof using HV. introv R. rewrite* <- @binds_equiv_read_opt in R. Qed.
-
-(** indom--read_opt **)
-
-Lemma not_indom_read_opt : forall h k,
-  ~ indom h k -> read_opt h k = None.
-Proof using HV. introv. erewrite not_indom_equiv_read_opt; autos*. Qed.
-
-Lemma read_opt_not_indom : forall h k,
-  read_opt h k = None -> ~ indom h k.
-Proof using HV. introv. erewrite not_indom_equiv_read_opt; autos*. Qed.
-
-End HeapFacts.
-
-
-
-
-
-
-Parameter indom_equiv_binds : forall h k,
-  indom h k = (exists v, binds h k v).
-
-Parameter dom_empty :
-  dom (@empty K V) = \{}.
-
-Parameter binds_equiv_read : forall h k,
-  indom h k -> (forall v, (binds h k v) = (read h k = v)).
-
-Parameter dom_write : forall h r v,
-  dom (write h r v) = dom h \u \{r}.
-
-Parameter binds_write_eq : forall h k v,
+Lemma binds_write_same : forall k v h,
   binds (write h k v) k v.
+Proof using. intros. rewrite binds_write_eq. case_if*. Qed.
 
-Parameter binds_write_neq : forall h k v k' v',
-  binds h k v -> k <> k' ->
+Lemma binds_write_neq : forall h k v k' v',
+  binds h k v ->
+  k <> k' ->
   binds (write h k' v') k v.
+Proof using. intros. rewrite binds_write_eq. case_if*. Qed.
 
-Parameter binds_write_inv : forall h k v k' v',
+Lemma binds_write_same_inv : forall h k v v',
+  binds (write h k v') k v ->
+  v = v'.
+Proof using. introv M. rewrite binds_write_eq in M. case_if*. Qed.
+
+Lemma binds_write_neq_inv : forall h k k' v v',
   binds (write h k' v') k v ->
-  (k = k' /\ v = v') \/ (k <> k' /\ binds h k v).
+  k <> k' ->
+  binds h k v.
+Proof using. introv M N. rewrite binds_write_eq in M. case_if*. Qed.
 
-Parameter binds_rem : forall h k k' v,
-  binds h k v -> k <> k' -> binds (rem h k') k v.
+(** Properties of [binds] on [rem] *)
 
-Parameter binds_rem_inv : forall h k v k',
-  binds (rem h k') k v -> k <> k' /\ binds h k v.
+Lemma binds_rem_eq : forall h k k' v,
+    binds (rem h k') k v
+  = (k <> k' /\ binds h k v).
+Proof using.
+  intros. extens. unfold binds. rewrite* read_opt_rem. repeat case_if*.
+Qed.
 
-Parameter not_indom_rem : forall h k,
-  ~ indom (rem h k) k.
+Lemma not_binds_rem_same : forall h k v,
+  ~ binds (rem h k) k v.
+Proof using. intros. rewrite binds_rem_eq. rew_logic*. Qed.
 
-Parameter binds_equiv_read_opt : forall `{Inhab V} h k v,
-  (binds h k v) = (read_opt h k = Some v).
+Lemma binds_rem : forall h k k' v,
+  binds h k v ->
+  k <> k' ->
+  binds (rem h k') k v.
+Proof using. intros. rewrite* binds_rem_eq. Qed.
 
-Parameter not_indom_equiv_read_opt : forall `{Inhab V} h k,
-  (~ indom h k) = (read_opt h k = None).
+Lemma binds_rem_inv : forall h k k' v,
+  binds (rem h k') k v ->
+  k <> k' /\ binds h k v.
+Proof using. introv M. rewrite* binds_rem_eq in M. Qed.
 
-Parameter read_opt_def : forall h k,
-  read_opt h k = (If indom h k then Some (read h k) else None).
-
-End HeapParameters.
-
-Arguments binds_equiv_read : clear implicits.
-
-Parameter indom_decidable : forall `{Comparable K} V (h:heap K V) k,
-  Decidable (indom h k).
-Existing Instance indom_decidable.
-
-End HeapSpec.
-
-
-(***********************************************************)
-(** Properties *)
+End HeapMoreProp.
 
 
-
-
-
-
-
-Arguments empty {K} {V}.
-
-Parameter binds : heap K V -> K -> V -> Prop.
-
-Definition indom h r :=	(r \in dom h).
-
-Parameter read : forall `{Comparable K} `{Inhab V}, heap K V -> K -> V.
-
-
-
-
-
-
-(***********************************************************)
-(** Properties *)
-
-Section HeapParameters.
-Context K (HK:Comparable K) V (HV:Inhab V).
-Implicit Types h : heap K V.
-
-Parameter indom_equiv_binds : forall h k,
-  indom h k = (exists v, binds h k v).
-
-Parameter dom_empty :
-  dom (@empty K V) = \{}.
-
-Parameter binds_equiv_read : forall h k,
-  indom h k -> (forall v, (binds h k v) = (read h k = v)).
-
-Parameter dom_write : forall h r v,
-  dom (write h r v) = dom h \u \{r}.
-
-Parameter binds_write_eq : forall h k v,
-  binds (write h k v) k v.
-
-Parameter binds_write_neq : forall h k v k' v',
-  binds h k v -> k <> k' ->
-  binds (write h k' v') k v.
-
-Parameter binds_write_inv : forall h k v k' v',
-  binds (write h k' v') k v ->
-  (k = k' /\ v = v') \/ (k <> k' /\ binds h k v).
-
-Parameter binds_rem : forall h k k' v,
-  binds h k v -> k <> k' -> binds (rem h k') k v.
-
-Parameter binds_rem_inv : forall h k v k',
-  binds (rem h k') k v -> k <> k' /\ binds h k v.
-
-Parameter not_indom_rem : forall h k,
-  ~ indom (rem h k) k.
-
-Parameter binds_equiv_read_opt : forall `{Inhab V} h k v,
-  (binds h k v) = (read_opt h k = Some v).
-
-Parameter not_indom_equiv_read_opt : forall `{Inhab V} h k,
-  (~ indom h k) = (read_opt h k = None).
-
-Parameter read_opt_def : forall h k,
-  read_opt h k = (If indom h k then Some (read h k) else None).
-
-End HeapParameters.
-
-Arguments binds_equiv_read : clear implicits.
-
-Parameter indom_decidable : forall `{Comparable K} V (h:heap K V) k,
-  Decidable (indom h k).
-Existing Instance indom_decidable.
-
-End HeapSpec.
+End Heap.
